low/RelationCorrect.v
@@ -2,5 +2,7 @@
  * Proof that the relation defined in Module Relation holds along the
  * execution of the functions of Reval. *)
 
+Require Export Relation.
+
 (* TODO *)
 
